module plfa.part1.Quantifiers where

import Relation.Binary.PropositionalEquality as Eq
open Eq using (_≡_; refl)
open import Data.Nat using (ℕ; zero; suc; _+_; _*_)
open import Relation.Nullary using (¬_)
open import Data.Product using (_×_; proj₁; proj₂) renaming (_,_ to ⟨_,_⟩)
open import Data.Sum using (_⊎_; inj₁; inj₂)
open import plfa.part1.Isomorphism using (_≃_; extensionality)

∀-elim : ∀ {A : Set} {B : A → Set}
  → (L : ∀ (x : A) → B x)
  → (M : A)
    -----------------
  → B M
∀-elim L M = L M

∀-distrib-× : ∀ {A : Set} {B C : A → Set} →
  (∀ (x : A) → B x × C x) ≃ (∀ (x : A) → B x) × (∀ (x : A) → C x)
∀-distrib-× = record
  {
    to = λ{ f → ⟨ (λ{ a → proj₁ (f a) })  , (λ{ b → proj₂ (f b) }) ⟩ } ; -- i don't know why???
    from = λ{ ⟨ f1 , f2 ⟩ → λ{ c → ⟨ f1 c , f2 c ⟩ } } ;
    to∘from = λ{ f → refl } ;
    from∘to = λ{ f → refl }
  }

data Σ (A : Set) (B : A → Set) : Set where
  ⟨_,_⟩ : (x : A) → B x → Σ A B

Σ-syntax = Σ
infix 2 Σ-syntax
syntax Σ-syntax A (λ x → B) = Σ[ x ∈ A ] B

record Σ′ (A : Set) (B : A → Set) : Set where
  field
    proj₁′ : A
    proj₂′ : B proj₁′

∃ : ∀ {A : Set} (B : A → Set) → Set
∃ {A} B = Σ A B

∃-syntax = ∃
syntax ∃-syntax (λ x → B) = ∃[ x ] B

∃-elim : ∀ {A : Set} {B : A → Set} {C : Set}
  → (∀ x → B x → C)
  → ∃[ x ] B x
    ---------------
  → C
∃-elim f ⟨ x , y ⟩ = f x y

∀∃-currying : ∀ {A : Set} {B : A → Set} {C : Set}
  → (∀ x → B x → C) ≃ (∃[ x ] B x → C)
∀∃-currying =
  record
    { to      =  λ{ f → λ{ ⟨ x , y ⟩ → f x y }}
    ; from    =  λ{ g → λ{ x → λ{ y → g ⟨ x , y ⟩ }}}
    ; from∘to =  λ{ f → refl }
    ; to∘from =  λ{ g → extensionality λ{ ⟨ x , y ⟩ → refl} }
    }

∃-distrib-⊎ : ∀ {A : Set} {B C : A → Set} →
  ∃[ x ] (B x ⊎ C x) ≃ (∃[ x ] B x) ⊎ (∃[ x ] C x)
∃-distrib-⊎ = record {
  to = λ{ ⟨ x , inj₁ y ⟩ → inj₁ ⟨ x , y ⟩ ; ⟨ x , inj₂ y ⟩ → inj₂ ⟨ x , y ⟩ } ;
  from = λ{ (inj₁ ⟨ x , y ⟩) → ⟨ x , inj₁ y ⟩; (inj₂ ⟨ x , y ⟩) →  ⟨ x , inj₂ y ⟩ } ;
  to∘from = λ{ (inj₁ ⟨ x , y ⟩) → refl ; (inj₂ ⟨ x , y ⟩) → refl} ;
  from∘to = λ{ ⟨ x , inj₁ y ⟩ → refl ; ⟨ x , inj₂ y ⟩ → refl}
  }

data even : ℕ → Set
data odd  : ℕ → Set

data even where

  even-zero : even zero

  even-suc : ∀ {n : ℕ}
    → odd n
      ------------
    → even (suc n)

data odd where
  odd-suc : ∀ {n : ℕ}
    → even n
      -----------
    → odd (suc n)

even-∃ : ∀ {n : ℕ} → even n → ∃[ m ] (    m * 2 ≡ n)
odd-∃  : ∀ {n : ℕ} →  odd n → ∃[ m ] (1 + m * 2 ≡ n)

even-∃ even-zero                       =  ⟨ zero , refl ⟩
even-∃ (even-suc o) with odd-∃ o
...                    | ⟨ m , refl ⟩  =  ⟨ suc m , refl ⟩

odd-∃  (odd-suc e)  with even-∃ e
...                    | ⟨ m , refl ⟩  =  ⟨ m , refl ⟩


∃-even : ∀ {n : ℕ} → ∃[ m ] (    m * 2 ≡ n) → even n
∃-odd  : ∀ {n : ℕ} → ∃[ m ] (1 + m * 2 ≡ n) →  odd n

∃-even ⟨  zero , refl ⟩  =  even-zero
∃-even ⟨ suc m , refl ⟩  =  even-suc (∃-odd ⟨ m , refl ⟩)

∃-odd  ⟨     m , refl ⟩  =  odd-suc (∃-even ⟨ m , refl ⟩)